Subtyping is completed.  Head for Typechecking and Record.

Subty.v
@@ -1,7 +1,9 @@
 Require Import SfLib.
-Require Import Maps.
+
 Require Import Types.
 Require Import STLCWA.
+
+Require Import LibTactics.
 
 
 Module Subtype.
@@ -13,6 +15,7 @@ Inductive ty : Type :=
     | TArrow : ty -> ty -> ty
     | TUnit : ty.
 
+    Hint Constructors ty.
 Inductive tm : Type :=
     | tvar : id -> tm 
     | tapp : tm -> tm -> tm
@@ -21,6 +24,8 @@ Inductive tm : Type :=
     | tfalse : tm 
     | tif : tm -> tm -> tm -> tm 
     | tunit : tm.
+    
+    Hint Constructors tm.
 
 
     Reserved Notation "x '<:' y" (at level 40).
@@ -43,8 +48,8 @@ Inductive tm : Type :=
                 x <: z
         where "x '<:' y" := (subtype_of x y).
 
-    
-    Reserved Notation "G '|=' x '\in' T" (at level 40).
+
+    Hint Constructors subtype_of.
 
     Fixpoint subst (i : id) (x org : tm) : tm :=
         match org with
@@ -58,7 +63,561 @@ Inductive tm : Type :=
     
     Notation "[ x ':=' s ] a" := (subst x s a) (at level 40).
 
-    Inductive has_type : 
+    Print tm.
+    Inductive has_type : Context -> tm -> ty -> Prop :=
+        | tyVar :
+            forall (i: id) G (T:ty),
+                byContext G i = Some T ->
+                has_type G (tvar i) T
+        | tyAbs :
+            forall i G x U T,
+                has_type (update i T G) x U ->
+                has_type G (tabs i T x) (TArrow T U)
+        | tyApp :
+            forall G abs arg U T,
+                has_type G abs (TArrow U T) ->
+                has_type G arg U ->
+                has_type G (tapp abs arg) T 
+        | tyTrue :
+            forall G,
+                has_type G ttrue TBool
+        | tyFalse :
+            forall G,
+                has_type G tfalse TBool
+        | tyUnit :
+            forall G,
+                has_type G tunit TUnit
+        | tyIf :
+            forall G x t0 t1 T,
+                has_type G t0 T ->
+                has_type G t1 T ->
+                has_type G x TBool ->
+                has_type G (tif x t0 t1) T
+        | tySub :
+            forall G x U V,
+                has_type G x U ->
+                U <: V ->
+                has_type G x V.
+
+    Notation "G '|=' x '\in' T" :=
+        (has_type G x T) (at level 40).
+
+    Hint Constructors has_type.
+
+    Inductive value : tm -> Prop :=
+        | vAbs : forall x T v, value (tabs x T v)
+        | vTrue : value ttrue
+        | vFalse : value tfalse
+        | vunit : value tunit.
+
+    Hint Constructors value.
+
+    Inductive step : tm -> tm -> Prop :=
+        | stApp0 :
+            forall a a' b,
+                step a a' ->
+                step (tapp a b) (tapp a' b)
+        | stApp1 :
+            forall a b b',
+                value a ->
+                step b b' ->
+                step (tapp a b) (tapp a b')
+        | stApp2 :
+            forall x T v b,
+                value b ->
+                step (tapp (tabs x T v) b) ([x := b] v)
+        | stIf0 :
+            forall x x' t0 t1,
+                step x x' ->
+                step (tif x t0 t1) (tif x' t0 t1)
+        | stIfTrue :
+            forall t0 t1,
+                step (tif ttrue t0 t1) t0
+        | stIfFalse :
+            forall t0 t1,
+                step (tif tfalse t0 t1) t1.
+    
+    Notation "a '==>' b" := (step a b) (at level 40).
+
+    Hint Constructors step.
+
+    Module EXAMPLES.
+        Notation x := (Id 0).
+        Notation y := (Id 1).
+        Notation z := (Id 2).
+
+        Notation A := (TBase (Id 6)).
+        Notation B := (TBase (Id 7)).
+        Notation C := (TBase (Id 8)).
+
+        Notation String := (TBase (Id 9)).
+        Notation Float := (TBase (Id 10)).
+        Notation Integer := (TBase (Id 11)).
+
+        Example subtyping_ex0: 
+            (TArrow C TBool) <: (TArrow C TTop).
+
+            eauto.
+        Qed.
+
+    End EXAMPLES.
+
+    Hint Extern 2 (has_type _ (tapp _ _) _) =>
+        eapply tyApp; auto.
+
+    Hint Extern 2 (_ = _) =>
+        compute; reflexivity.
+
+    Module EXAMPLES2.
+    Import EXAMPLES.
+    End EXAMPLES2.
+
+Lemma sub_inversion_Bool :
+        forall U,
+            U <: TBool ->
+            U = TBool.
+
+        intros U h. 
+        remember TBool as t.
+        induction h; subst. inversion Heqt.
+        inversion Heqt. auto. 
+        pose (IHh2 eq_refl).
+        pose (IHh1 e). rewrite e0; rewrite e. auto.
+        
+Qed.
+
+Lemma sub_inversion_arrow :
+    forall U V1 V2,
+        (U <: (TArrow V1 V2)) ->
+        exists U1 U2,
+            (U = TArrow U1 U2) /\
+            (V1 <: U1) /\
+            (U2 <: V2).
+
+    intros u v1 v2 h.
+    remember (TArrow v1 v2) as v.
+    generalize dependent v1; generalize dependent v2.
+    induction h; subst; intros; try discriminate.
+    inversion Heqv; subst.
+    exists x; exists y; tauto.
+    exists v1; exists v2; repeat (split; eauto).
+    destruct (IHh2 _ _ Heqv) as (u1 & u2 & H1 & H2 & H3); subst.
+    destruct (IHh1 u2 u1 eq_refl) as (a1 & a2 & a3 & a4 &a5).
+    exists a1; exists a2; try tauto.
+    repeat (split; eauto).
+Qed. 
+
+Lemma canonical_form_of_arrow_ty :
+    forall Gamma s T1 T2,
+        Gamma |= s \in (TArrow T1 T2) ->
+        value s ->
+        exists x S1 s2,
+            s = tabs x S1 s2.
+        
+    intros G s T1 T2 h1.
+    remember (TArrow T1 T2) as Ar.
+    gen T1 T2.
+    induction h1; eauto;
+    try (intros T1 T2 h0 hh; inversion hh; fail);
+    try (intros T1 T2 h0; inversion h0; fail).
+    
+    intros; subst.
+    destruct (sub_inversion_arrow _ _ _ H) as (u1 & u2 & hh1 & hh2 & hh3).
+    eauto.
+Qed.
+
+Lemma canonical_form_of_bool_ty :
+    forall G s,
+        G |= s \in TBool ->
+        value s ->
+        s = ttrue \/ s = tfalse.
+
+    intros G s h. remember TBool as t.
+    gen Heqt.
+    induction h; eauto;
+    try (intros hh1 hh2; inversion hh2; fail);
+    try (intros hh1; inversion hh1; fail).
+
+    intros; subst. 
+    pose (sub_inversion_Bool _ H).
+    eauto.
+Qed.
+
+
+Ltac go_far :=
+    match goal with
+        | [x: ?pre -> _ |- _] => 
+                    (assert (pre) as GO_FAR_H; 
+                    [eauto; fail | eauto];
+                    pose (x GO_FAR_H) as GO_FAR_HH; 
+                        generalize GO_FAR_HH; 
+                        try (clear GO_FAR_HH); 
+                        try (clear GO_FAR_H);
+                        clear x; intro x; go_far
+                            )
+        | _ => idtac 
+    end.
+
+
+Theorem progress:
+    forall x T,
+        empty |= x \in T ->
+        value x \/ exists x', x ==> x'.
+
+    intros x T h.
+    remember empty as eg.
+    gen Heqeg. 
+    induction h; try (intros; subst; eauto).
+    inversion H.
+    destruct (IHh1 eq_refl). destruct (IHh2 eq_refl).
+    destruct (canonical_form_of_arrow_ty _ _ _ _ h1 H) as (x & S1 &s2 & hh); subst.
+    right; exists ([x := arg] s2); eauto.
+    destruct H0 as (arg' & hh);
+    right; exists (tapp abs arg'); eauto.
+    destruct H as (abs' & hh); right ;exists (tapp abs' arg); eauto.
+    go_far.
+    destruct IHh3. 
+    destruct (canonical_form_of_bool_ty _ _ h3 H); subst.
+    right; exists t0; eauto.
+    right; exists t1; eauto.
+    destruct H as (x'0 & H); subst;
+    right; exists (tif x'0 t0 t1); eauto.
+
+Qed.
+
+Lemma typing_inversion_abs :
+    forall G x S1 t2 T,
+        G |= tabs x S1 t2 \in T ->
+        (exists S2, (TArrow S1 S2) <: T /\
+            (update x S1 G) |= t2 \in S2).
+
+    intros G x S1 t2 T h.
+    remember (tabs x S1 t2) as v.
+    gen x S1 t2.
+    induction h; intros x0 S1 t2 h0; subst; eauto;
+    try (inversion h0; subst; eauto; fail).
+
+    destruct (IHh x0 S1 t2) as (S3 & hh & hhh); eauto.
+Qed.
+
+Lemma typing_inversion_var :
+    forall G x T ,
+        G |= tvar x \in T ->
+        exists S,
+            byContext G x = Some S /\
+            S <: T.
+
+    intros G x T h.
+    remember (tvar x) as v.
+    gen x.
+
+    induction h; try (intros; subst; eauto; fail);
+    try (intros a h' ; subst; inversion h'; fail);
+    intros a h'; subst.
+    inversion h'; subst; eauto.
+    destruct (IHh a eq_refl ) as (S & h0 & h1); eauto.
+Qed.
+
+Lemma typing_inversion_app0 :
+    forall G t1 t2 T,
+        G |= (tapp t1 t2) \in T ->
+        (exists S1 S2, G |= t1 \in TArrow S1 S2 /\
+        G |= t2 \in S1 /\
+        S2 <: T).
+
+        intros G t1 t2 T2 h1.
+        remember (tapp t1 t2) as v.
+        gen t1 t2.
+
+        induction h1; try (intros; subst; eauto;fail);
+        try (intros t1 t2 h0; subst; inversion h0; fail);
+        intros a1 a2 h0; subst.
+
+        inversion h0; subst. eauto.
+        inversion h0; subst.
+        destruct (IHh1 a1 a2 eq_refl) as (S1 & S2 & H0 & H1 & H2).
+        exists S1; exists S2; eauto.
+Qed.
+
+Lemma typing_inversion_app :
+    forall G t1 t2 T2,
+        G |= (tapp t1 t2) \in T2 ->
+        (exists T1, 
+            G |= t1 \in TArrow T1 T2 /\
+            G |= t2 \in T1).
+    
+    intros G t1 t2 T2 h;
+    remember (tapp t1 t2) as v;
+    gen t1 t2;
+    induction h; try (intros; subst; eauto ;fail );
+    try (intros t1 t2 hh; subst; inversion hh; subst ;fail).
+
+    intros. inversion Heqv; subst. eauto.
+    intros t2 t3 hh; inversion hh.
+    intros. destruct (IHh _ _ Heqv) as (T1 & h1 & h2); eauto.
+Qed.
+
+Lemma typing_inversion_true :
+    forall G T,
+        G |= ttrue \in T ->
+        TBool <: T.
+
+    intros G T h; 
+    remember ttrue as v;
+    gen Heqv.
+    induction h; try (intros h; subst; inversion h; eauto; fail).
+    intros. inversion Heqv. eauto.
+Qed.
+
+Lemma typing_inversion_if :
+    forall G t1 t2 t3 T,
+        G |= tif t1 t2 t3 \in T ->
+        G |= t1 \in TBool /\
+        (exists S, G |= t2 \in S /\
+                    G |= t3 \in S /\
+                        S <: T).
+
+    intros G t1 t2 t3 T h;
+    remember (tif t1 t2 t3) as v;
+    gen t1 t2 t3.
+    induction h; try (intros t1 t2 t3 hh; inversion hh; subst; eauto).
+
+    intros t2 t3 t4 hh. inversion hh; subst. eauto.
+    destruct (IHh t1 t2 t3 eq_refl) as (S & h0 & h1 & h2 & h3); eauto.
+    split; eauto.
+Qed.   
+
+Lemma typing_inversion_false :
+    forall G T,
+        G |= tfalse \in T ->
+        TBool <: T.
+
+        intros G T h; 
+        remember tfalse as v;
+        gen Heqv.
+        induction h; try (intros h; subst; inversion h; eauto; fail).
+        intros. inversion Heqv. eauto.
+Qed.
+
+
+Lemma typing_inversion_unit:
+    forall G T,
+         G |= tunit \in T ->
+         TUnit <: T.
+
+         intros G T h; 
+         remember tunit as v;
+         gen Heqv.
+         induction h; try (intros h; subst; inversion h; eauto; fail).
+         intros. inversion Heqv. eauto.
+Qed.
+
+
+Lemma abs_arrow :
+    forall x S1 s2 T1 T2,
+        empty |= tabs x S1 s2 \in (TArrow T1 T2) ->
+        T1 <: S1 /\
+        (update x S1 empty) |= s2 \in T2.
+
+    intros x S1 s2 T1 T2 h1.
+    destruct (typing_inversion_abs _ _ _ _ _ h1) as 
+        (S2 & hh & hhh).
+    destruct (sub_inversion_arrow _ _ _ hh) as 
+            (u1 & u2 & hh1 & hh2 & hh3).
+    inversion hh1; subst; eauto.
+Qed.
+
+Print tm.
+
+Inductive occurs_free : id -> tm -> Prop :=
+    | of_var : forall i,
+                occurs_free i (tvar i)
+    | of_app1 : forall i x y,
+                occurs_free i x ->
+                occurs_free i (tapp x y)
+    | of_app2 : forall i x y,
+                occurs_free i y ->
+                occurs_free i (tapp x y)
+    | of_abs : forall i x T v,
+                i <> x ->
+                occurs_free i v ->
+                occurs_free i (tabs x T v)
+    | of_if0 : forall i t t0 t1,
+                occurs_free i t ->
+                occurs_free i (tif t t0 t1)
+    | of_if1 : forall i t t0 t1,
+                occurs_free i t0 ->
+                occurs_free i (tif t t0 t1)
+    | of_if2 : forall i t t0 t1,
+                occurs_free i t1 ->
+                occurs_free i (tif t t0 t1).
+
+    Hint Constructors occurs_free.
+
+Hint Resolve typing_inversion_abs typing_inversion_var
+            typing_inversion_app typing_inversion_true
+            typing_inversion_false typing_inversion_if
+            typing_inversion_unit abs_arrow : inv_ty_db.
+
+Ltac typing_inversion_auto :=
+    match goal with
+        | [x : _ |= tvar _ \in _  |- _] => destruct (typing_inversion_var _ _ _ x) as (ss0 & hh0 & hh1)
+        | [x : _ |= tapp _ _ \in _ |- _] => destruct (typing_inversion_app _ _ _ _ x) as (ss0 & hh0 & hh1)
+        | [x : _ |= tabs _ _ _ \in TArrow _ _ |- _] => destruct (abs_arrow _ _ _ _ _ x) as ( hh0 & hh1)  
+        | [x : _ |= tabs _ _ _ \in _ |- _] => destruct (typing_inversion_abs _ _ _ _ _ x) as (ss0 & hh0 & hh1)
+        | [x : _ |= ttrue \in _ |- _] => pose (typing_inversion_true _ _ x) as hh0
+        | [x : _ |= tfalse \in _ |- _] => pose (typing_inversion_false _ _ x) as hh0
+        | [x : _ |= tunit \in _ |- _] => pose (typing_inversion_unit _ _ x) as hh0
+        | [x : _ |= tif _ _ _ \in _ |- _] => destruct (typing_inversion_if _ _ _ _ _ x) as (ss0 & hh0 & hh1 & hh2 & hh3)
+        | _ => idtac
+    end; eauto.
+Lemma occurs_free_in_ctx :
+    forall G i t T,
+        occurs_free i t ->
+        G |= t \in T ->
+        (exists S, byContext G i = Some S).
+    
+    intros G i t T h.
+    gen G T.
+    induction h; try (subst; intros; typing_inversion_auto; eauto with inv_ty_db).
+    destruct (IHh _ _ hh1) as (S & h0). cbn in *.
+    destruct (eq_id_dec i x); subst; eauto.
+    destruct (H eq_refl).
+Qed.
+
+
+Lemma context_invariance :
+    forall G G' t S,
+        G |= t \in S ->
+        (forall x, occurs_free x t -> byContext G x = byContext G' x) ->
+        G' |= t \in S.
+
+    intros G G' t S h.
+    gen G'.
+    induction h; intros; typing_inversion_auto.
+
+    intros. eapply tyVar.
+    rewrite <- H0; eauto.
+    
+    intros; eauto. eapply tyAbs.
+    assert (forall x0, occurs_free x0 x -> byContext (update i T G) x0 = byContext (update i T G') x0).
+    cbn. intros. destruct (eq_id_dec x0 i); subst; eauto.
+    eauto.
+
+    eapply tyIf; eauto.
+Qed.
+
+
+
+
+Lemma empty_is_closed :
+    forall x T,
+        empty |= x \in T ->
+        (forall i, ~occurs_free i x).
+
+    intros x T h1 i h2.
+    gen T h1.
+    induction h2; subst; intros; typing_inversion_auto.
+
+    inversion hh0. 
+    assert (occurs_free i (tabs x T v)); eauto.
+    destruct  (occurs_free_in_ctx _ _ _ _ H0 h1) as (S & hh);
+    inversion hh.
+Qed.
+
+Lemma empty_is_strong :
+    forall x G T,
+        empty |= x \in T ->
+        G |= x \in T.
+
+    intros. eapply context_invariance; eauto.
+    intros x0 hh. destruct (empty_is_closed _ _ H x0 hh).
+Qed.
+
+
+Theorem ctx_swap :
+    forall U V t T,
+        U |= t \in T ->
+        U =-= V ->
+        V |= t \in T.
+    intros U V t; gen U V.
+    induction t;
+    try (unfold context_equivalence; intros; typing_inversion_auto; fail); try (intros; typing_inversion_auto).
+
+    intros; unfold context_equivalence in *; typing_inversion_auto; eapply tySub; try eapply hh1. eapply tyVar. rewrite <- H0; eauto.
+    eapply tySub; try eapply hh0. eapply tyAbs.  eapply IHt. eapply hh1.
+    eapply update_inc; eapply H0.
+    eapply tyIf; eauto.
+Qed.
+
+Lemma subst_preserve_typing:
+forall G x U g t S,
+    (update x U G) |= t \in S ->
+    empty |= g \in U ->
+    G |= [x := g] t \in S.
+
+intros G x U g t.
+gen G x U g.
+induction t; cbn in *; intros; typing_inversion_auto; cbn in *.
+destruct (eq_id_dec x i); subst; eauto. rewrite eq_id_dec_id in *. inversion hh0; subst.
+eapply empty_is_strong. eauto.
+destruct (eq_id_dec i x); subst; eauto. destruct (n eq_refl).
+destruct (eq_id_dec x i); subst; eauto. 
+eapply tySub; try eapply hh0. eapply tyAbs; eauto. 
+eapply ctx_swap; try eapply hh1. eapply update_shadow. eapply refl_ctxeq.
+eapply tySub; try eapply hh0. eapply tyAbs; eauto. eapply IHt; eauto.
+eapply ctx_swap; try eapply hh1; try eapply update_permute; eauto.
+eapply refl_ctxeq.
+eapply tyIf; eauto.
+Qed.
+
+
+Theorem preservation:
+    forall t t' T,
+        empty |= t \in T ->
+        t ==> t' ->
+        empty |= t' \in T.
+
+    intro t; induction t;
+     try (intros t' T h1 h2; inversion h2; subst; typing_inversion_auto).
+
+    typing_inversion_auto.
+
+    destruct (abs_arrow _ _ _ _ _ hh0).
+    eapply subst_preserve_typing; eauto.
+Qed.
+
+(* Corollary  Soundness is omitted. *)
+
+End Subtype.
+
+
+
+
+
+
+
+
+
+    
+
+
+
+
+
+
+
+
+    
+
+
+
+
+
+
+
+
+    
 
     
         
